src/lang/Thread.v
@@ -133,13 +133,20 @@ Module Thread.
     .
     Hint Constructors opt_step.
 
+    Definition steps_abort (e1: t): Prop :=
+      exists e2 e3,
+        <<STEPS: rtc tau_step e1 e2>> /\
+        <<ABORT: step true ThreadEvent.abort e2 e3>>.
+    Hint Unfold steps_abort.
+
     Definition consistent (e:t): Prop :=
       forall mem1 sc1
         (CAP: Memory.cap e.(local).(Local.promises) e.(memory) mem1)
         (SC_MAX: Memory.max_full_timemap mem1 sc1),
-      exists e2,
-        <<STEPS: rtc tau_step (mk e.(state) e.(local) sc1 mem1) e2>> /\
-        <<PROMISES: e2.(local).(Local.promises) = Memory.bot>>.
+        <<ABORT: steps_abort (mk e.(state) e.(local) sc1 mem1)>> \/
+        exists e2,
+          <<STEPS: rtc tau_step (mk e.(state) e.(local) sc1 mem1) e2>> /\
+          <<PROMISES: e2.(local).(Local.promises) = Memory.bot>>.
 
 
     (* step_future *)
