src/while/Semantics.v
@@ -99,6 +99,22 @@ Module RegFile.
         (Instr.syscall lhs rhses)
         (ProgramEvent.syscall (Event.mk lhs_val (map (eval_value rf) rhses)))
         (RegFun.add lhs lhs_val rf)
+  | eval_assert_success
+      rf e
+      (ASSERT: eval_expr rf e <> 0):
+      eval_instr
+        rf
+        (Instr.assert e)
+        (ProgramEvent.silent)
+        rf
+  | eval_assert_fail
+      rf e
+      (ASSERT: eval_expr rf e = 0):
+      eval_instr
+        rf
+        (Instr.assert e)
+        (ProgramEvent.abort)
+        rf
   .
 
   Definition eq_except (regs:RegSet.t) (rs_src rs_tgt:RegFile.t): Prop :=
@@ -254,6 +270,10 @@ Module RegFile.
         unfold RegFun.add, RegFun.find. condtac; auto.
       + ii. eapply REGS; eauto.
         apply RegSet.add_spec. auto.
+    - erewrite <- eq_except_expr in ASSERT; eauto.
+      esplits; eauto. econs. auto.
+    - erewrite <- eq_except_expr in ASSERT; eauto.
+      esplits; eauto. econs. auto.
   Qed.
 
   Lemma instr_ord_eval_instr
